\iffalse
\documentclass[journal,12pt,twocolumn]{IEEEtran}
\usepackage{setspace}
\usepackage{gensymb}
\singlespacing
\usepackage[cmex10]{amsmath}
\usepackage{amsthm}
\usepackage{mathrsfs}
\usepackage{txfonts}
\usepackage{stfloats}
\usepackage{bm}
\usepackage{cite}
\usepackage{cases}
\usepackage{subfig}
\usepackage{longtable}
\usepackage{multirow}
\usepackage{enumitem}
\usepackage{mathtools}
\usepackage{tikz}
\usepackage{circuitikz}
\usepackage{verbatim}
\usepackage[breaklinks=true]{hyperref}
\usepackage{tkz-euclide} % loads  TikZ and tkz-base
\usepackage{listings}
\usepackage{color}    
\usepackage{array}    
\usepackage{longtable}
\usepackage{calc}     
\usepackage{multirow} 
\usepackage{hhline}   
\usepackage{ifthen}   
\usepackage{lscape}     
\usepackage{chngcntr}
\DeclareMathOperator*{\Res}{Res}
\renewcommand\thesection{\arabic{section}}
\renewcommand\thesubsection{\thesection.\arabic{subsection}}
\renewcommand\thesubsubsection{\thesubsection.\arabic{subsubsection}}

\renewcommand\thesectiondis{\arabic{section}}
\renewcommand\thesubsectiondis{\thesectiondis.\arabic{subsection}}
\renewcommand\thesubsubsectiondis{\thesubsectiondis.\arabic{subsubsection}}
\renewcommand\thetable{\arabic{table}}
% correct bad hyphenation here
\hyphenation{op-tical net-works semi-conduc-tor}
\def\inputGnumericTable{}                                 %%

\lstset{
%language=C,
frame=single, 
breaklines=true,
columns=fullflexible
}
%\lstset{
%language=tex,
%frame=single, 
%breaklines=true
%}

\begin{document}
\newtheorem{theorem}{Theorem}[section]
\newtheorem{problem}{Problem}
\newtheorem{proposition}{Proposition}[section]
\newtheorem{lemma}{Lemma}[section]
\newtheorem{corollary}[theorem]{Corollary}
\newtheorem{example}{Example}[section]
\newtheorem{definition}[problem]{Definition}
\newcommand{\BEQA}{\begin{eqnarray}}
\newcommand{\EEQA}{\end{eqnarray}}
\newcommand{\define}{\stackrel{\triangle}{=}}
\bibliographystyle{IEEEtran}
\providecommand{\mbf}{\mathbf}
\providecommand{\pr}[1]{\ensuremath{\Pr\left(#1\right)}}
\providecommand{\qfunc}[1]{\ensuremath{Q\left(#1\right)}}
\providecommand{\sbrak}[1]{\ensuremath{{}\left[#1\right]}}
\providecommand{\lsbrak}[1]{\ensuremath{{}\left[#1\right.}}
\providecommand{\rsbrak}[1]{\ensuremath{{}\left.#1\right]}}
\providecommand{\brak}[1]{\ensuremath{\left(#1\right)}}
\providecommand{\lbrak}[1]{\ensuremath{\left(#1\right.}}
\providecommand{\rbrak}[1]{\ensuremath{\left.#1\right)}}
\providecommand{\cbrak}[1]{\ensuremath{\left\{#1\right\}}}
\providecommand{\lcbrak}[1]{\ensuremath{\left\{#1\right.}}
\providecommand{\rcbrak}[1]{\ensuremath{\left.#1\right\}}}
\theoremstyle{remark}
\newtheorem{rem}{Remark}
\newcommand{\sgn}{\mathop{\mathrm{sgn}}}
\providecommand{\abs}[1]{\left\vert#1\right\vert}
\providecommand{\res}[1]{\Res\displaylimits_{#1}} 
\providecommand{\norm}[1]{\left\lVert#1\right\rVert}
\providecommand{\mtx}[1]{\mathbf{#1}}
\providecommand{\mean}[1]{E\left[ #1 \right]}
\providecommand{\fourier}{\overset{\mathcal{F}}{ \rightleftharpoons}}
\providecommand{\system}[1]{\overset{\mathcal{#1}}{ \longleftrightarrow}}
\newcommand{\solution}{\noindent \textbf{Solution: }}
\newcommand{\cosec}{\,\text{cosec}\,}
\providecommand{\dec}[2]{\ensuremath{\overset{#1}{\underset{#2}{\gtrless}}}}
\newcommand{\myvec}[1]{\ensuremath{\begin{pmatrix}#1\end{pmatrix}}}
\newcommand{\mydet}[1]{\ensuremath{\begin{vmatrix}#1\end{vmatrix}}}
\let\vec\mathbf
\def\putbox#1#2#3{\makebox[0in][l]{\makebox[#1][l]{}\raisebox{\baselineskip}[0in][0in]{\raisebox{#2}[0in][0in]{#3}}}}
     \def\rightbox#1{\makebox[0in][r]{#1}}
     \def\centbox#1{\makebox[0in]{#1}}
     \def\topbox#1{\raisebox{-\baselineskip}[0in][0in]{#1}}
     \def\midbox#1{\raisebox{-0.5\baselineskip}[0in][0in]{#1}}

\vspace{3cm}
\title{Probability Assignment}
\author{Gautam Singh}
\maketitle
\bigskip

\begin{abstract}
    This document contains the solution to Question 21 of 
    Exercise 3 in Chapter 16 of the class 11 NCERT textbook.
\end{abstract}

\begin{enumerate}
   
    \solution 
		\fi
		Define random variables $X$ and $Y$ as shown
    in Tables \ref{tab:ncert/11/16/3/21/X-def} and \ref{tab:ncert/11/16/3/21/Y-def}.
    \begin{table}[!ht]
        \centering
        \input{ncert/11/16/3/21/tables/11.16.03.21_1.tex}
        \caption{Definition of $X$.}
        \label{tab:ncert/11/16/3/21/X-def}
    \end{table}
    \begin{table}[!ht]
        \centering
        \input{ncert/11/16/3/21/tables/11.16.03.21_2.tex}
        \caption{Definition of $Y$.}
        \label{tab:ncert/11/16/3/21/Y-def}
    \end{table}
    From the given data
    \begin{align}
        \pr{X=1} &= \frac{30}{60} = \frac{1}{2} \label{eq:ncert/11/16/3/21/pr-X} \\
        \pr{Y=1} &= \frac{32}{60} = \frac{8}{15} \label{eq:ncert/11/16/3/21/pr-Y} \\
        \pr{X=1,\ Y=1} &= \frac{24}{60} = \frac{2}{5} \label{eq:ncert/11/16/3/21/pr-XY}
    \end{align}
    Thus, we write
    \begin{align}
	    \pr{X=1,\ Y=0}         &= \pr{X=1} - \pr{X=1,\ Y=1} = \frac{1}{10} \\
	    \pr{X=0,\ Y=1}        &= \pr{Y=1} - \pr{X=1,\ Y=1} = \frac{2}{15} \\
        \pr{X=0,\ Y=0} 
        &= \pr{Y=0} - \pr{X=1,\ Y=0} 
	\\
	    &= 1 - \pr{Y=1} - \pr{X=1,\ Y=0} \\
        &= 1 - \frac{8}{15} - \frac{1}{10} = \frac{11}{30}
    \end{align}
    and form the joint pmf as in Table \ref{tab:ncert/11/16/3/21/joint}.
    \begin{table}[!ht]
        \centering
        \input{ncert/11/16/3/21/tables/11.16.03.21_3.tex}
        \caption{Joint pmf of $X$ and $Y$.}
        \label{tab:ncert/11/16/3/21/joint}
    \end{table}
    \begin{enumerate}
        \item From Table 
        \ref{tab:ncert/11/16/3/21/joint},
        \begin{align}
            \pr{X+Y\ge1} &= 1 - \pr{X+Y=0} \\
                         &= \frac{19}{30}
        \end{align}
        
        \item From Table \ref{tab:ncert/11/16/3/21/joint},
        \begin{align}
\pr{X=0,\ Y=0} = \frac{11}{30}
\end{align}

        \item From Table \ref{tab:ncert/11/16/3/21/joint},
        \begin{align}
\pr{X=0,\ Y=1} = \frac{2}{15}
\end{align}
    \end{enumerate}
